concurrency/erased_machine.v
@@ -111,7 +111,7 @@ Module ErasedMachineShell (SEM:Semantics)  <: ConcurrentMachineSig
        forall (tp' : thread_pool) c m' b ofs
          (Hcode: getThreadC cnt0 = Kblocked c)
          (Hat_external: at_external Sem c =
-                        Some (LOCK, ef_sig LOCK, Vptr b ofs::nil))
+                        Some (LOCK, Vptr b ofs::nil))
          (Hload: Mem.load Mint32 m b (Int.intval ofs) = Some (Vint Int.one))
          (Hstore: Mem.store Mint32 m b (Int.intval ofs) (Vint Int.zero) = Some m')
          (Htp': tp' = updThreadC cnt0 (Kresume c Vundef)),
@@ -121,7 +121,7 @@ Module ErasedMachineShell (SEM:Semantics)  <: ConcurrentMachineSig
        forall (tp':thread_pool) c m' b ofs
          (Hcode: getThreadC cnt0 = Kblocked c)
          (Hat_external: at_external Sem c =
-                        Some (UNLOCK, ef_sig UNLOCK, Vptr b ofs::nil))
+                        Some (UNLOCK, Vptr b ofs::nil))
          (Hstore: Mem.store Mint32 m b (Int.intval ofs) (Vint Int.one) = Some m')
          (Htp': tp' = updThreadC cnt0 (Kresume c Vundef)),
          ext_step genv cnt0 Hcompat tp' m' (release (b, Int.intval ofs) None)
@@ -130,7 +130,7 @@ Module ErasedMachineShell (SEM:Semantics)  <: ConcurrentMachineSig
        forall (tp_upd tp':thread_pool) c b ofs arg
          (Hcode: getThreadC cnt0 = Kblocked c)
          (Hat_external: at_external Sem c =
-                        Some (CREATE, ef_sig CREATE, Vptr b ofs::arg::nil))
+                        Some (CREATE, Vptr b ofs::arg::nil))
          (Htp_upd: tp_upd = updThreadC cnt0 (Kresume c Vundef))
          (Htp': tp' = addThread tp_upd (Vptr b ofs) arg tt),
          ext_step genv cnt0 Hcompat tp' m (spawn (b, Int.intval ofs))
@@ -139,7 +139,7 @@ Module ErasedMachineShell (SEM:Semantics)  <: ConcurrentMachineSig
        forall  (tp': thread_pool) c m' b ofs
           (Hcode: getThreadC cnt0 = Kblocked c)
           (Hat_external: at_external Sem c =
-                         Some (MKLOCK, ef_sig MKLOCK, Vptr b ofs::nil))
+                         Some (MKLOCK, Vptr b ofs::nil))
           (Hstore: Mem.store Mint32 m b (Int.intval ofs) (Vint Int.zero) = Some m')
           (Htp': tp' = updThreadC cnt0 (Kresume c Vundef)),
          ext_step genv cnt0 Hcompat tp' m' (mklock (b, Int.intval ofs))
@@ -148,7 +148,7 @@ Module ErasedMachineShell (SEM:Semantics)  <: ConcurrentMachineSig
        forall (tp' tp'': thread_pool) c b ofs
          (Hcode: getThreadC cnt0 = Kblocked c)
          (Hat_external: at_external Sem c =
-                        Some (FREE_LOCK, ef_sig FREE_LOCK, Vptr b ofs::nil))
+                        Some (FREE_LOCK, Vptr b ofs::nil))
          (Htp': tp' = updThreadC cnt0 (Kresume c Vundef)),
          ext_step genv cnt0 Hcompat  tp' m (freelock (b,Int.intval ofs))
                   
@@ -156,7 +156,7 @@ Module ErasedMachineShell (SEM:Semantics)  <: ConcurrentMachineSig
        forall  c b ofs
           (Hcode: getThreadC cnt0 = Kblocked c)
           (Hat_external: at_external Sem c =
-                         Some (LOCK, ef_sig LOCK, Vptr b ofs::nil))
+                         Some (LOCK, Vptr b ofs::nil))
           (Hload: Mem.load Mint32 m b (Int.intval ofs) = Some (Vint Int.zero)),
          ext_step genv cnt0 Hcompat tp m (failacq (b, Int.intval ofs)).
    
