concurrency/semax_conc.v
@@ -532,7 +532,7 @@ Theorem oracular_refinement cs ext_link ge n oracle c m :
   jsafeN (Concurrent_Oracular_Espec cs ext_link).(@OK_spec) ge n oracle c m.
 Proof.
   revert oracle c m; induction n as [n InductionHypothesis] using strong_nat_ind; intros oracle c m.
-  intros Safe; induction Safe as [ | | n z_unit c m e sig args x E Pre Post | ].
+  intros Safe; induction Safe as [ | | n z_unit c m e args x E Pre Post | ].
   all: swap 3 4.
   - (* safeN_0 *)
     now eapply safeN_0; eauto.
@@ -545,8 +545,8 @@ Proof.
     now eapply safeN_halted; eauto.
   
   - (* safeN_external *)
-    destruct c as [ | ef_ sig_ args_ lid ve te k ]; [ discriminate | ].
-    simpl in E; injection E as -> -> -> .
+    destruct c as [ | ef_ args_ lid ve te k ]; [ discriminate | ].
+    simpl in E; injection E as -> -> .
     
     (* We need to know which of the externals we are talking about *)
     (* paragraph below: ef has to be an EF_external *)
@@ -597,7 +597,7 @@ Proof.
                forall x2 : T,
                  @JMeq (rmap * (Prop * list rmap * val * share * Pred)) xwith T x2 ->
                  @jsafeN (list rmap) (concurrent_oracular_ext_spec cs ext_link) ge (S n) nil
-                         (Clight_new.ExtCall (EF_external name sg) sig args lid ve te k) m)
+                         (Clight_new.ExtCall (EF_external name sg) args lid ve te k) m)
               (@ext_spec_type juicy_mem external_function (@OK_ty (Concurrent_Oracular_Espec cs ext_link))
                               (@OK_spec (Concurrent_Oracular_Espec cs ext_link)) (EF_external name sg))).
         {
@@ -673,7 +673,7 @@ Proof.
                forall x2 : T,
                  @JMeq (rmap * (Prop * list rmap * val * share * Pred)) xwith T x2 ->
                  @jsafeN (list rmap) (concurrent_oracular_ext_spec cs ext_link) ge (S n) (phi_oracle :: oracle)
-                         (Clight_new.ExtCall (EF_external name sg) sig args lid ve te k) m)
+                         (Clight_new.ExtCall (EF_external name sg) args lid ve te k) m)
               (@ext_spec_type juicy_mem external_function (@OK_ty (Concurrent_Oracular_Espec cs ext_link))
                               (@OK_spec (Concurrent_Oracular_Espec cs ext_link)) (EF_external name sg))).
         {
@@ -755,7 +755,7 @@ Proof.
              forall x2 : T,
                @JMeq (rmap * (list rmap * val * share * Pred)) xwith T x2 ->
                @jsafeN (list rmap) (concurrent_oracular_ext_spec cs ext_link) ge (S n) oracle
-                       (Clight_new.ExtCall (EF_external name sg) sig args lid ve te k) m)
+                       (Clight_new.ExtCall (EF_external name sg) args lid ve te k) m)
             (@ext_spec_type juicy_mem external_function (@OK_ty (Concurrent_Oracular_Espec cs ext_link))
                             (@OK_spec (Concurrent_Oracular_Espec cs ext_link)) (EF_external name sg))).
       {
