progs/verif_even.v
@@ -80,7 +80,7 @@ Lemma all_funcs_correct: semax_func Vprog Gprog (prog_funct prog) Gprog.
 Proof.
 unfold Gprog, prog, prog_funct.
 simpl.
- repeat (apply semax_func_cons_ext_vacuous; [reflexivity | ]);
+ repeat (apply semax_func_cons_ext_vacuous; [reflexivity | reflexivity | ]);
 semax_func_cons_ext. renormalize.
  apply (temp_make_ext_rval_e gx (Vint (if Z.odd z then Int.one else Int.zero)) ret) in H;
   try congruence.
